sets

src/Std/Data/ExtTreeSet/Basic.lean
@@ -191,6 +191,13 @@ def getD [TransCmp cmp] (t : ExtTreeSet α cmp) (a : α) (fallback : α) : α :=
   t.inner.getKeyD a fallback
 
 /--
+Checks if given key is contained and returns the key if it is, otherwise returns `Classical.ofNonempty`.
+If the key is contained the result is guaranteed to be pointer equal to the key in the set.
+-/
+noncomputable def getV [TransCmp cmp] [Nonempty α] (t : ExtTreeSet α cmp) (a : α) : α :=
+  t.getD a Classical.ofNonempty
+
+/--
 Tries to retrieve the smallest element of the tree set, returning `none` if the set is empty.
 -/
 @[inline]
